Implement n secret sharing

Additive.ec
@@ -1,17 +1,24 @@
 
 require import DBool.
+require import Int.
+require import List.
+
+
+
 
 require import PrimeField.
 
 type Share = t.
 type Secret = t.
 
-module type Protocol = {
+
+module type Protocol2 = {
   proc share(secret: Secret): Share * Share
   proc reconstruct(shares: Share * Share): Secret
 }.
 
-module AdditiveSecretShare: Protocol = {
+
+module AdditiveSecret2Share: Protocol2 = {
 
   proc share(secret : Secret): Share * Share = {
     var share1, share2;
@@ -21,19 +28,6 @@ module AdditiveSecretShare: Protocol = {
     share2 <- secret - share1;
 
     return (share1, share2);
-  }
-
-  (* I didn't know how to get the first share in the lemma so just made this*)
-  proc fst_share(secret : Secret): Share = {
-    var share1, share2;
-    (share1, share2) <@ share(secret);
-    return share1;
-  }
-
-  proc fst_share_is_value(secret : Secret, expected_share : Share): bool = {
-    var share1, share2;
-    (share1, share2) <@ share(secret);
-    return (share1 = expected_share);
   }
 
   proc reconstruct(shares : Share * Share): Secret = {
@@ -48,22 +42,55 @@ module AdditiveSecretShare: Protocol = {
 
 }.
 
+(* This works but maybe is not the best way*)
+(* Given two secrets and a share. The probability the first shares of each match a given share is equal. *)
+lemma additive_secret_share2 &m (secret1 : Secret) (secret2 : Secret) (a: Share) :
+    Pr [ AdditiveSecret2Share.share(secret1) @ &m : fst res = a ] =
+    Pr [ AdditiveSecret2Share.share(secret2) @ &m : fst res = a ].
+proof.
+admit.
+qed.
+
+(* Now let's extend it to n shares *)
+
+(* A data structure to always ensure that there are two shares *)
+type shares = [ LastTwoShares of Share & Share | ShareCons of Share & shares].
+
+(* Example of construction*)
+op lastTwo = LastTwoShares (ofint 3) (ofint 2).
+op allShares = ShareCons (ofint 4) lastTwo.
+
+module type ProtocolN = {
+  proc share(secret: Secret, n: int): shares
+  (*proc reconstruct(shares: shares): Secret*)
+}.
+
+module AdditiveSecretnShare: ProtocolN = {
+
+  proc share(secret : Secret, n: int): shares = {
+    var share1, share2, total;
+    var shares_l : shares;
+
+    while (2 <= n) {
+      share1 <$ FDistr.dt;
+      if (n = 2) {
+        share2 <- secret - total;
+        shares_l <- LastTwoShares share1 share2;
+      }
+      else {
+        shares_l <- ShareCons share1 shares_l;
+      }
+    }
+    return shares_l;
+  }
+
+}.
+
 (* How do we get the first element? Like this: *)
 lemma test_fst : fst (3, 2) = 3.
 proof.
 trivial.
 qed.
-
-
-(* This works but maybe is not the best way*)
-(* Given two secrets and a share. The probability the first shares of each match a given share is equal. *)
-lemma additive_secret_share2 &m (secret1 : Secret) (secret2 : Secret) (a: Share) :
-    Pr [ AdditiveSecretShare.share(secret1) @ &m : fst res = a ] =
-    Pr [ AdditiveSecretShare.share(secret2) @ &m : fst res = a ].
-
-(* I think this doesn't work for us*)
-lemma additive_secret_share4 &m (secret1 : Secret) (secret2 : Secret) (a: Share) :
-    equiv [ AdditiveSecretShare.share ~ AdditiveSecretShare.share : ={A} ==> res{1} = res{2} ].
 
 
 
@@ -73,5 +100,3 @@ lemma additive_secret_share4 &m (secret1 : Secret) (secret2 : Secret) (a: Share)
 (*&m is memory*)
 (*res is result*)
 (*So this states given some memory &m G1.f() and G2.f() return true at about the same rate*)
-lemma G1_G2_true &m :
-Pr[G1.f() @ &m : res] = Pr[G2.f() @ &m : res].
